verify/Indv1.v
@@ -10,7 +10,7 @@ Import Inductive62.
 Ltac solve_hlin_nonhalt_T T :=
   apply (decide_hlin_nonhalt_spec default_config T);
   [ apply Config_WF_simple; reflexivity
-  | vm_cast_no_check (eq_refl true)].
+  | native_cast_no_check (eq_refl true)].
 
 Ltac solve_hlin_nonhalt :=
   match goal with
