verify/RWLAcc.v
@@ -1,0 +1,546 @@
+Require Import NArith.
+Require Import List.
+Require Import Lia.
+From BusyCoq Require Import DHTM.
+From BusyCoq Require Import Eqb.
+
+Ltac destruct_spec_expr e f :=
+match e with
+| match ?a with _ => _ end => destruct_spec_expr a f
+| if ?a then _ else _ => destruct_spec_expr a f
+| ?a ?arg1 ?arg2 ?arg3 ?arg4 ?arg5 ?arg6 ?arg7 =>
+  pose proof (f arg1 arg2 arg3 arg4 arg5 arg6 arg7);
+  destruct e
+| ?a ?arg1 ?arg2 ?arg3 ?arg4 ?arg5 ?arg6 =>
+  pose proof (f arg1 arg2 arg3 arg4 arg5 arg6);
+  destruct e
+| ?a ?arg1 ?arg2 ?arg3 ?arg4 ?arg5 =>
+  pose proof (f arg1 arg2 arg3 arg4 arg5);
+  destruct e
+| ?a ?arg1 ?arg2 ?arg3 ?arg4 =>
+  pose proof (f arg1 arg2 arg3 arg4);
+  destruct e
+| ?a ?arg1 ?arg2 ?arg3 =>
+  pose proof (f arg1 arg2 arg3);
+  destruct e
+| ?a ?arg1 ?arg2 =>
+  pose proof (f arg1 arg2);
+  destruct e
+| ?a ?arg1 =>
+  pose proof (f arg1);
+  destruct e
+end.
+
+Ltac destruct_spec f :=
+match goal with
+|- ?a => destruct_spec_expr a f
+end.
+
+Module RWLAcc(Ctx:Ctx).
+Module DHTM := DHTM Ctx.
+Export DHTM.
+Section bsz.
+Hypothesis tm:TM.
+Hypothesis bsz bmaxT:nat.
+Definition RW:Type := (list Sym)*N*N.
+Definition RWL:Type := list RW.
+Definition RWL_config:Type := RWL*RWL*Q*dir.
+
+Definition pop(ls:RWL):option ((list Sym)*RWL) :=
+match ls with
+| [] => Some (repeat s0 bsz,[])
+| (w,a,Npos b)::t =>
+  let b':=Pos.pred_N b in
+  match b' with
+  | N0 =>
+    match a with
+    | N0 => Some (w,t)
+    | _ => None
+    end
+  | _ => Some (w,(w,a,b')::t)
+  end
+| _ => None
+end.
+
+Definition push(w:list Sym)(ls:RWL):RWL :=
+match ls with
+| [] => (w,0,1)%N::nil
+| (w',a,b)::t =>
+  if eqb w w' then
+    (w,a,N.succ b)::t
+  else
+    (w,0,1)%N::ls
+end.
+
+Definition push'(x:RW)(ls:RWL):RWL :=
+let '(w,a,b):=x in
+match ls with
+| (w',a',b')::t =>
+  if eqb w w' then
+    (w',a+a',b+b')%N::t
+  else x::ls
+| _ => x::ls
+end.
+
+Fixpoint match_side(ls1 ls2:RWL):option RWL :=
+match ls1,ls2 with
+| (w1,N0,b1)::t1,(w2,N0,b2)::t2 =>
+  if (eqb w1 w2) && (b1 <=? b2)%N then
+    match_side t1 t2 &&& (fun t0 => Some ((w1,b2-b1,b1)%N::t0))
+  else None
+| nil,nil => Some nil
+| _,_ => None
+end.
+
+Definition match_config(c1 c2:RWL_config):option RWL_config :=
+let '(l1,r1,s1,sgn1):=c1 in
+let '(l2,r2,s2,sgn2):=c2 in
+if (eqb s1 s2) && (eqb sgn1 sgn2) then
+  match_side l1 l2 &&& (fun l0 =>
+  match_side r1 r2 &&& (fun r0 =>
+  Some (l0,r0,s1,sgn1)
+  ))
+else None.
+
+Definition RWL_step(c:RWL_config):option RWL_config :=
+let '(l,r,s,sgn):=c in
+pop l &&& (fun '(l0,l1) =>
+pop r &&& (fun '(r0,r1) =>
+DH_cconfig_bounded_progress tm (l0,r0,s,sgn) bmaxT &&& (fun '(l0',r0',s',sgn') =>
+match r0' with
+| nil =>
+let l0a := firstn bsz l0' in
+let l0b := skipn bsz l0' in
+if eqb sgn sgn' then
+if eqb s s' && eqb l0 l0a then
+match r with
+| nil => None
+| (w,a,b)::t =>
+  if eqb r0 w then
+  match b with
+  | Npos _ => Some (push l0a (push' (l0b,a,b) l1),t,s',sgn')
+  | _ => None
+  end
+  else None
+end
+else Some (push l0a (push l0b l1),r1,s',sgn')
+else Some (push l0a (push l0b r1),l1,s',sgn')
+| _ => None
+end
+))).
+
+Definition RWL_step''(c:RWL_config*bool):RWL_config*bool+unit :=
+let (c,_):=c in
+match RWL_step c with
+| None => inr tt
+| Some c' => inl (c',true)
+end.
+
+Definition side_subst_S(ls:RWL):RWL :=
+map (fun '(w,a,b) => (w,a,a+b)%N) ls.
+
+Definition side_subst_O(ls:RWL):RWL :=
+map (fun '(w,a,b) => (w,0,b)%N) ls.
+
+Definition config_subst_S(c:RWL_config):RWL_config :=
+let '(l,r,s,sgn):=c in
+(side_subst_S l,side_subst_S r,s,sgn).
+
+Definition config_subst_O(c:RWL_config):RWL_config :=
+let '(l,r,s,sgn):=c in
+(side_subst_O l,side_subst_O r,s,sgn).
+
+Definition check_nonhalt c1 c2 n :=
+match match_config c1 c2 with
+| None => false
+| Some c3 =>
+  match N_iter_until RWL_step'' (inl (c3,false)) n with
+  | inl (c4,true) => eqb (config_subst_S c3) c4 && eqb (config_subst_O c3) c1
+  | _ => false
+  end
+end.
+
+Definition RWL_state:Type := RWL_config*RWL_config*N*N.
+Definition RWL_step'(x:RWL_state):RWL_state+bool :=
+let '(c1,c,n,n0):=x in
+match RWL_step c with
+| None => inr false
+| Some c' =>
+  if (n <? n0)%N then
+    if check_nonhalt c1 c' (N.succ n) then inr true
+    else inl (c1,c',N.succ n,n0)
+  else
+    inl (c',c',N0,n0*2)%N
+end.
+
+Definition RWL_state_0:RWL_state := ((([],[],q0,R),([],[],q0,R),0,1)%N).
+
+Definition RWL_steps T :=
+N_iter_until RWL_step' (inl RWL_state_0) T.
+
+Section subst_i.
+Hypothesis i:nat.
+
+Definition to_seg(x:RW) :=
+let '(w,a,b):=x in
+w ^^ ((N.to_nat a)*i+(N.to_nat b)).
+
+Definition to_side(ls:RWL) := (flat_map to_seg ls) *> Streams.const s0.
+
+Definition to_config(c:RWL_config):DH_config :=
+let '(l,r,s,sgn):=c in
+(to_side l,to_side r,s,sgn).
+
+Lemma push_spec w ls:
+  to_side (push w ls) =
+  w *> to_side ls.
+Proof.
+  destruct ls as [|[[w' a'] b'] t].
+  - cbn.
+    rewrite Str_app_assoc.
+    cbn.
+    change (Pos.to_nat 1) with 1.
+    cbn.
+    rewrite Str_app_assoc.
+    reflexivity.
+  - cbn - [eqb].
+    destruct (eqb_spec w w').
+    + cbn.
+      repeat rewrite Str_app_assoc.
+      replace (N.to_nat a' * i + N.to_nat (N.succ b')) with (S(N.to_nat a' * i + N.to_nat b')) by lia.
+      cbn.
+      rewrite Str_app_assoc.
+      subst.
+      reflexivity.
+    + cbn.
+      repeat rewrite Str_app_assoc.
+      change (Pos.to_nat 1) with 1.
+      cbn.
+      rewrite Str_app_assoc.
+      reflexivity.
+Qed.
+
+Lemma push'_spec x ls:
+  to_side (push' x ls) =
+  to_seg x *> to_side ls.
+Proof.
+  destruct x as [[w a] b].
+  destruct ls as [|[[w' a'] b'] t].
+  - cbn.
+    rewrite Str_app_assoc.
+    reflexivity.
+  - cbn - [eqb].
+    destruct (eqb_spec w w').
+    + cbn.
+      repeat rewrite Str_app_assoc.
+      replace (N.to_nat (a + a') * i + N.to_nat (b + b')) with ((N.to_nat a * i + N.to_nat b)+(N.to_nat a' * i + N.to_nat b')) by lia.
+      rewrite lpow_add.
+      rewrite Str_app_assoc.
+      subst.
+      reflexivity.
+    + cbn.
+      repeat rewrite Str_app_assoc.
+      reflexivity.
+Qed.
+
+Lemma pop_spec ls:
+match pop ls with
+| None => True
+| Some (x,t) =>
+  to_side ls =
+  x *> to_side t
+end.
+Proof.
+  destruct ls as [|[[w a] b] t].
+  - cbn.
+    induction bsz.
+    1: reflexivity.
+    cbn. rewrite <-IHn,<-const_unfold.
+    reflexivity.
+  - cbn.
+    destruct b as [|b]; trivial.
+    destruct (Pos.pred_N b) eqn:E.
+    + cbn.
+      repeat rewrite Str_app_assoc.
+      assert (b=1)%positive by lia.
+      subst b.
+      change (Pos.to_nat 1) with 1.
+      destruct a as [|a]; trivial.
+      cbn.
+      rewrite Str_app_assoc.
+      reflexivity.
+    + cbn.
+      replace (N.to_nat a * i + Pos.to_nat b) with (S(N.to_nat a * i + Pos.to_nat p)) by lia.
+      cbn.
+      repeat rewrite Str_app_assoc.
+      reflexivity.
+Qed.
+
+Lemma to_side_def a b:
+  to_side (a::b) = to_seg a *> to_side b.
+Proof.
+  cbn.
+  rewrite Str_app_assoc.
+  reflexivity.
+Qed.
+
+Lemma RWL_step_spec c:
+match RWL_step c with
+| None => True
+| Some c' => (to_config c) -[ tm ]->+ (to_config c')
+end.
+Proof.
+  destruct c as [[[l r] s] sgn].
+  unfold RWL_step.
+  unfold if_Some.
+  destruct_spec pop_spec; trivial.
+  destruct p as [l0 l1].
+  destruct_spec pop_spec; trivial.
+  destruct p as [r0 r1].
+  destruct_spec DH_cconfig_bounded_progress_spec; trivial.
+  destruct p as [[[l0' r0'] s'] sgn'].
+  destruct H1 as [H1 H2].
+  cbn in H2.
+  unfold to_config.
+  rewrite H,H0.
+  destruct r0'; trivial.
+  destruct (eqb_spec sgn sgn').
+  - destruct sgn,sgn'; try congruence; (
+      destruct (eqb_spec s s');
+      [| shelve];
+      destruct (eqb_spec l0 (firstn bsz l0'));
+      [| shelve];
+      destruct r as [|[[w a] b] r]; trivial;
+      destruct (eqb_spec r0 w); trivial;
+      rewrite <-H0;
+      destruct b as [|b]; trivial;
+      rewrite to_side_def;
+      rewrite push_spec;
+      rewrite push'_spec;
+      unfold to_seg;
+      remember (N.to_nat a * i + N.to_nat (N.pos b)) as v1;
+      rewrite <-(firstn_skipn bsz l0') in H2;
+      subst l0;
+      remember (firstn bsz l0') as l0a;
+      remember (skipn bsz l0') as l0b;
+      destruct v1 as [|v1]; try lia;
+      clear Heqv1;
+      generalize (to_side r) as r';
+      generalize (to_side l1) as l';
+      subst r0 s;
+      induction v1; intros;
+      [ epose proof (H2 _ _) as H2;
+        rewrite Str_app_assoc in H2;
+        cbn in H2;
+        cbn[lpow];
+        repeat rewrite app_nil_r;
+        apply H2
+      | remember (S v1) as v2;
+        epose proof (H2 _ _) as H2;
+        rewrite Str_app_assoc in H2;
+        cbn in H2;
+        cbn[lpow];
+        repeat rewrite Str_app_assoc;
+        eapply progress_trans;
+        [ apply H2
+        | applys_eq IHv1;
+           do 4 f_equal;
+           repeat rewrite <-Str_app_assoc;
+           f_equal;
+           rewrite lpow_shift;
+           reflexivity ] ]).
+  - destruct sgn,sgn'; try congruence;
+    shelve.
+Unshelve.
+all:
+      unfold to_config;
+      do 2 rewrite push_spec;
+      rewrite <-(firstn_skipn bsz l0') in H2;
+      applys_eq H2;
+      rewrite Str_app_assoc;
+      reflexivity.
+Qed.
+End subst_i.
+
+Lemma RWL_step_spec' c:
+match RWL_step c with
+| None => True
+| Some c' => forall i, (to_config i c) -[ tm ]->+ (to_config i c')
+end.
+Proof.
+  destruct (RWL_step c) eqn:E; trivial.
+  intros i.
+  pose proof (RWL_step_spec i c) as H.
+  rewrite E in H.
+  apply H.
+Qed.
+
+Lemma side_subst_S_spec i ls:
+  to_side i (side_subst_S ls) = to_side (S i) ls.
+Proof.
+  unfold to_side,side_subst_S.
+  induction ls.
+  1: reflexivity.
+  cbn.
+  repeat rewrite Str_app_assoc.
+  rewrite IHls.
+  f_equal.
+  destruct a as [[w a] b].
+  cbn.
+  f_equal. lia.
+Qed.
+
+Lemma side_subst_O_spec i ls:
+  to_side i (side_subst_O ls) = to_side 0 ls.
+Proof.
+  unfold to_side,side_subst_O.
+  induction ls.
+  1: reflexivity.
+  cbn.
+  repeat rewrite Str_app_assoc.
+  rewrite IHls.
+  f_equal.
+  destruct a as [[w a] b].
+  cbn.
+  f_equal. lia.
+Qed.
+
+Lemma config_subst_S_spec i c:
+  to_config i (config_subst_S c) = to_config (S i) c.
+Proof.
+  destruct c as [[[l r] s] sgn].
+  cbn.
+  repeat rewrite side_subst_S_spec.
+  reflexivity.
+Qed.
+
+Lemma config_subst_O_spec i c:
+  to_config i (config_subst_O c) = to_config O c.
+Proof.
+  destruct c as [[[l r] s] sgn].
+  cbn.
+  repeat rewrite side_subst_O_spec.
+  reflexivity.
+Qed.
+
+Lemma nonhalt_cond c:
+  c0 -[ tm ]->* (to_config 0 c) ->
+  (forall i, to_config i c -[ tm ]->+ to_config (S i) c) ->
+  ~halts tm c0.
+Proof.
+  intros.
+  eapply evstep_nonhalt.
+  2: apply H.
+  eapply progress_nonhalt with (P:=fun c' => exists i, c' = to_config i c).
+  2: eexists; reflexivity.
+  intros c1 [i Hc1].
+  subst c1.
+  eexists _.
+  split.
+  2: apply (H0 i).
+  eexists; reflexivity.
+Qed.
+
+Lemma RWL_step''_spec c n:
+match N_iter_until RWL_step'' (inl (c,false)) n with
+| inl (c',flag) =>
+  if flag then
+    (forall i, to_config i c -[ tm ]->+ to_config i c')
+  else c=c'
+| inr _ => True
+end.
+Proof.
+  eapply N_iter_until_spec.
+  2: reflexivity.
+  intros [c1 flag1] H.
+  unfold RWL_step''.
+  destruct flag1.
+  - destruct_spec (RWL_step_spec'); trivial.
+    intros i.
+    eapply progress_trans; eauto.
+  - destruct_spec (RWL_step_spec'); trivial.
+    subst c1.
+    apply H0. 
+Qed.
+
+Lemma check_nonhalt_spec c1 c2 n:
+  c0 -[ tm ]->* (to_config 0 c1) ->
+  if check_nonhalt c1 c2 n then ~halts tm c0 else True.
+Proof.
+  intros Hc1.
+  unfold check_nonhalt.
+  destruct (match_config c1 c2) as [c3|]; trivial.
+  pose proof (RWL_step''_spec c3 n) as Hc4.
+  destruct (N_iter_until RWL_step'' (inl (c3, false)) n) as [[c4 [|]]|]; trivial.
+  destruct (eqb_spec (config_subst_S c3) c4); trivial.
+  destruct (eqb_spec (config_subst_O c3) c1); trivial.
+  rewrite <-e in Hc4.
+  apply (nonhalt_cond c3).
+  2: intros i; applys_eq Hc4.
+  2: rewrite config_subst_S_spec; reflexivity.
+  erewrite <-config_subst_O_spec.
+  rewrite e0.
+  apply Hc1.
+Qed.
+
+Definition RWL_state_WF(x:RWL_state) :=
+let '(c1,c2,_,_) := x in
+  c0 -[ tm ]->* to_config 0 c1 /\
+  c0 -[ tm ]->* to_config 0 c2.
+
+Lemma RWL_step'_spec x0 T:
+RWL_state_WF x0 ->
+match N_iter_until RWL_step' (inl x0) T with
+| inr flag =>
+  if flag then ~halts tm c0 else True
+| inl x1 => RWL_state_WF x1
+end.
+Proof.
+  intros Hx0.
+  eapply N_iter_until_spec.
+  2: apply Hx0.
+  intros [[[c1 c2] n1] n2].
+  unfold RWL_step'.
+  intros [Hc1 Hc2].
+  destruct_spec (RWL_step_spec O); trivial.
+  destruct (n1 <? n2)%N.
+  2: cbn; split;
+    apply progress_evstep; eapply evstep_progress_trans; eauto.
+  destruct_spec check_nonhalt_spec.
+  1: tauto.
+  cbn.
+  split. 1: tauto.
+  apply progress_evstep.
+  eapply evstep_progress_trans; eauto.
+Qed.
+
+Lemma RWL_state_0_WF:
+RWL_state_WF RWL_state_0.
+Proof.
+  cbn; split; constructor.
+Qed.
+
+Definition decide_nonhalt T :=
+match RWL_steps T with
+| inr true => true
+| _ => false
+end.
+
+Lemma decide_nonhalt_spec T:
+  decide_nonhalt T = true ->
+  ~halts tm c0.
+Proof.
+  unfold decide_nonhalt,RWL_steps.
+  pose proof (RWL_step'_spec RWL_state_0 T) as H0.
+  intros H.
+  destruct (N_iter_until RWL_step' (inl RWL_state_0) T).
+  1: congruence.
+  destruct b.
+  2: congruence.
+  apply H0,RWL_state_0_WF.
+Qed.
+
+End bsz.
+
+End RWLAcc.
+
