verify/Ternary.v
@@ -1,0 +1,171 @@
+Require Import NArith.
+Require Import PeanoNat.
+Require Import Lia.
+From BusyCoq Require Import LibTactics.
+
+Inductive ternary :=
+| xH0 | xH1
+| m3a2(x:ternary)
+| m3a3(x:ternary)
+| m3a4(x:ternary)
+.
+
+Fixpoint to_nat(x:ternary):nat :=
+match x with
+| xH0 => 0%nat
+| xH1 => 1%nat
+| m3a2 x0 => 2+(to_nat x0)*3
+| m3a3 x0 => 3+(to_nat x0)*3
+| m3a4 x0 => 4+(to_nat x0)*3
+end.
+
+Fixpoint of_nat'(x sz:nat): ternary :=
+match x with
+| 0 => xH0
+| 1 => xH1
+| S (S x) =>
+  match sz with
+  | 0 => xH0
+  | S sz =>
+    match x mod 3 with
+    | 0 => m3a2 (of_nat' (x/3) sz)
+    | 1 => m3a3 (of_nat' (x/3) sz)
+    | 2 => m3a4 (of_nat' (x/3) sz)
+    | _ => xH0
+    end
+  end
+end.
+
+Definition of_nat(x:nat): ternary := of_nat' x x.
+
+Lemma of_nat'_spec x sz:
+  x <= sz ->
+  of_nat' x sz = of_nat x.
+Proof.
+  gen sz.
+  induction x using Wf_nat.lt_wf_ind.
+  intros sz Hsz.
+  destruct x as [|[|x]].
+  1,2: destruct sz; reflexivity.
+  destruct sz as [|sz].
+  1: lia.
+  cbn[of_nat'].
+  pose proof (Nat.Div0.div_mod x 3) as Hx.
+  unshelve epose proof (Nat.mod_upper_bound x 3 _) as Hx2.
+  1: lia.
+  remember (x/3) as x1.
+  remember (x mod 3) as x2.
+  unfold of_nat.
+  replace (S x) with (x+1) by lia.
+  cbn[of_nat'].
+  replace (x+1) with (S x) by lia.
+  rewrite <-Heqx1,<-Heqx2.
+  destruct x2 as [|[|[|x2]]].
+  4: lia.
+  all: erewrite H; try lia;
+    erewrite H; try lia;
+    reflexivity.
+Qed.
+
+Lemma to_of_nat x:
+  to_nat (of_nat x) = x.
+Proof.
+  induction x using Wf_nat.lt_wf_ind.
+  destruct x as [|[|x]].
+  1,2: reflexivity.
+  pose proof (Nat.Div0.div_mod x 3) as Hx.
+  unshelve epose proof (Nat.mod_upper_bound x 3 _) as Hx2.
+  1: lia.
+  remember (x/3) as x1.
+  remember (x mod 3) as x2.
+  unfold of_nat.
+  replace (S x) with (x+1) by lia.
+  cbn[of_nat'].
+  replace (x+1) with (S x) by lia.
+  rewrite <-Heqx1,<-Heqx2.
+  destruct x2 as [|[|[|x2]]].
+  4: lia.
+  all: cbn[to_nat];
+    rewrite of_nat'_spec; try lia;
+    erewrite H; try lia.
+Qed.
+
+Lemma of_nat_m3a2 n:
+  of_nat (2+n*3) = m3a2 (of_nat n).
+Proof.
+  change (of_nat (2+n*3)) with (of_nat' (S (S (n*3))) (S (1+n*3))).
+  cbn[of_nat'].
+  rewrite Nat.Div0.mod_mul.
+  rewrite Nat.div_mul. 2: lia.
+  rewrite of_nat'_spec. 2: lia.
+  reflexivity.
+Qed.
+
+Lemma of_nat_m3a3 n:
+  of_nat (3+n*3) = m3a3 (of_nat n).
+Proof.
+  change (of_nat (3+n*3)) with (of_nat' (S (S (1+n*3))) (S (2+n*3))).
+  cbn[of_nat'].
+  rewrite Nat.Div0.mod_add.
+  change (1 mod 3) with 1.
+  cbn match.
+  rewrite Nat.div_add. 2: lia.
+  change (1 / 3) with 0.
+  rewrite of_nat'_spec. 2: lia.
+  reflexivity.
+Qed.
+
+Lemma of_nat_m3a4 n:
+  of_nat (4+n*3) = m3a4 (of_nat n).
+Proof.
+  change (of_nat (4+n*3)) with (of_nat' (S (S (2+n*3))) (S (3+n*3))).
+  cbn[of_nat'].
+  rewrite Nat.Div0.mod_add.
+  change (2 mod 3) with 2.
+  cbn match.
+  rewrite Nat.div_add. 2: lia.
+  change (2 / 3) with 0.
+  rewrite of_nat'_spec. 2: lia.
+  reflexivity.
+Qed.
+
+Fixpoint succ x :=
+match x with
+| xH0 => xH1
+| xH1 => m3a2 xH0
+| m3a2 x0 => m3a3 x0
+| m3a3 x0 => m3a4 x0
+| m3a4 x0 => m3a2 (succ x0)
+end.
+
+Lemma succ_spec x:
+  of_nat (S x) = succ (of_nat x).
+Proof.
+  induction x using Wf_nat.lt_wf_ind.
+  destruct x as [|[|x]].
+  1,2: reflexivity.
+  pose proof (Nat.Div0.div_mod x 3) as Hx.
+  unshelve epose proof (Nat.mod_upper_bound x 3 _) as Hx2.
+  1: lia.
+  remember (x/3) as x1.
+  remember (x mod 3) as x2.
+  destruct x2 as [|[|[|x2]]].
+  4: lia.
+  - replace (S(S(S x))) with (3+x1*3). 2: lia.
+    replace (S(S x)) with (2+x1*3). 2: lia.
+    rewrite of_nat_m3a3.
+    rewrite of_nat_m3a2.
+    reflexivity.
+  - replace (S(S(S x))) with (4+x1*3). 2: lia.
+    replace (S(S x)) with (3+x1*3). 2: lia.
+    rewrite of_nat_m3a4.
+    rewrite of_nat_m3a3.
+    reflexivity.
+  - replace (S(S(S x))) with (2+(S x1)*3). 2: lia.
+    replace (S(S x)) with (4+x1*3). 2: lia.
+    rewrite of_nat_m3a2.
+    rewrite of_nat_m3a4.
+    rewrite H. 2: lia.
+    reflexivity.
+Qed.
+
